
# Unit 01: The Riemann-Stieltjes integral

### Objectives

After studying this unit, students will be able to:
* define upper and lower Riemann-Stieltjes integral
* describe the condition of Riemann-Stieltjes integrability in terms of upper and lower Riemann-Stieltjes integral
* establish relation between Riemann-Stieltjes integral and Riemann integral
* define necessary and sufficient condition for Riemann-Stieltjes integrability
* understand theorems related to Riemann-Stieltjes integrability

### Introduction

Riemann-Stieltjes integral is the generalization of Riemann integral. It is based on the definition of Riemann integral. For the sake of convenience, we are giving the definition and preliminaries of Riemann integral.

## 1.1 Definition and Existence of the Integral

**Definition:** Let $f:[a,b]\rightarrow\mathbb{R}$ be a bounded function and
$P=\{a=x_{0},x_{1},x_{2},...,x_{n}\}$
be the partition of [a, b] such that $x_{0}\le x_{1}\le x_{2}\le\cdot\cdot\cdot\le x_{n}$.

If P and $p^{*}$ be the partition of the interval [a, b] such that $p^{*}\supset p$ then $p^{*}$ is known as the refinement of P.

If $P_{1}\cup P_{2}=P$ then P is the common refinement for $P_{1}$ and $P_{2}$.
We write
$m_{i}=inff(x),x_{i-1}\le x\le x_{i}$
$M_{i}=sup~f(x)$, $x_{i-1}\le x\le x_{i}$

$m\le f(x)\le M$ $\forall x\in[a,b]$, and
$\Delta x_{i}=x_{i}-x_{i-1}$
$\Rightarrow\Delta x_{i}\ge0$

$\sum_{i=1}^{n}\Delta x_{i}=\Delta x_{1}+\Delta x_{2}+\cdot\cdot\cdot+\Delta x_{n}$
$=x_{n}-x_{0}$
Thus, we get,
$\sum_{i=1}^{n}\Delta x_{i}=b-a$
Put
$$L(\mathcal{P},f)=\sum_{i=1}^{n}m_{i}\Delta x_{i},$$
$$U(\mathcal{P},f)=\sum_{i=1}^{n}M_{i}\Delta x_{i},$$
and finally
$$sup_{\mathfrak{P}}L(\mathcal{P},f)=\int_{\underline{a}}^{b}f(x)dx$$
$$inf_{\mathcal{P}}U(\mathcal{P},f)=\int_{a}^{\overline{b}}f(x)dx$$

If
$$\int_{\underline{a}}^{b}f(x)dx=\int_{a}^{\overline{b}}f(x)dx$$
Then fis Riemann integrable and we write $f\in\mathcal{R}$ and the common value is written as
$$\int_{a}^{b}f(x)dx$$
Now,
$m\le m_{i}\le M_{i}\le M$
$\sum_{i=1}^{n}m\Delta~x_{i}\le\sum_{i=1}^{n}m_{i}\Delta x_{i}\le\sum_{i=1}^{n}M_{i}\Delta x_{i}\le\sum_{i=1}^{n}M\Delta x_{i}$
$m\sum_{i=1}^{n}\Delta x_{i}\le L(P,f)\le U(P,f)\le M\sum_{i=1}^{n}\Delta x_{i}$
$\Rightarrow m(b-a)\le L(P,f)\le U(P,f)\le M(b-a)$

Thus, the numbers $L(P,f)$ and $U(P,f)$ form a bounded set which shows that upper and lower integrals are defined for every bounded functionf. Under what circumstances these two integrals are equal? This is a delicate issue. Instead of handling it separately for Riemann integral, we will consider now the more general case.

## 1.2 The Riemann -Stieltjes Integral

Let $f:[a,b]\rightarrow\mathbb{R}$ be a bounded function and $\alpha$ is a monotonically increasing function.
Corresponding to the partition $P=\{a=x_{0},x_{1},x_{2},...,x_{n}\}$ of [a, b] such that $x_{0}\le x_{1}\le x_{2}\le\cdot\cdot\cdot\le x_{n}$
we define
$\Delta\alpha_{i}=\alpha(x_{i})-\alpha(x_{i-1})\forall i$
$\Rightarrow\Delta\alpha_{i}\ge0$ as $\alpha$ is monotonically increasing.
$\sum_{i=1}^{n}\Delta\alpha_{i}=\Delta\alpha_{1}+\Delta\alpha_{2}+\cdot\cdot\cdot+\Delta\alpha_{n}$
$=[\alpha(x_{1})-\alpha(x_{0})]+[\alpha(x_{2})-\alpha(x_{1})]+\cdot\cdot\cdot+[\alpha(x_{n})-\alpha(x_{n-1})]$
$=\alpha(x_{n})-\alpha(x_{0})$
$=\alpha(b)-\alpha(a)$

Further, we put
$$L(P,f,\alpha)=\sum_{i=1}^{n}m_{i}\Delta\alpha_{i},m_{i}=inff(x),x_{i-1}\le x\le x_{i}$$
$$U(\mathcal{P},f,\alpha)=\sum_{i=1}^{n}M_{i}\Delta\alpha_{i},M_{i}=sup~f(x),x_{i-1}\le x\le x_{i}$$
$\Rightarrow L(P,f,\alpha)\le U(P,f,\alpha)$

We define,
$$sup_{\mathcal{P}}L(\mathcal{P},f,\alpha)=\int_{\underline{a}}^{b}fd\alpha$$
$\Rightarrow\int_{\underline{a}}^{b}fd\alpha\ge L(\mathcal{P},f,\alpha)$
and
$$inf_{\mathcal{P}}U(\mathcal{P},f,\alpha)=\int_{a}^{\overline{b}}fd\alpha$$
$\Rightarrow\int_{a}^{\overline{b}}fd\alpha\le U(\mathcal{P},f,\alpha)$
Now,
$m\le m_{i}\le M_{i}\le M$
$\sum_{i=1}^{n}m\Delta\alpha_{i}\le\sum_{i=1}^{n}m_{i}\Delta\alpha_{i}\le\sum_{i=1}^{n}M_{i}\Delta\alpha_{i}\le\sum_{i=1}^{n}M\Delta\alpha_{i}$
$m\sum_{i=1}^{n}\Delta\alpha_{i}\le L(P,f,\alpha)\le U(P,f,\alpha)\le M\sum_{i=1}^{n}\Delta\alpha_{i}$
$\Rightarrow m[\alpha(b)-\alpha(a)]\le L(P,f,\alpha)\le U(P,f,\alpha\le M[\alpha(b)-\alpha(a)].$

Now if
$$\int_{\underline{a}}^{b}fd\alpha=\int_{a}^{\overline{b}}fd\alpha,$$
then we denote their common value by
$$\int_{a}^{b}fd\alpha$$
or
$$\int_{a}^{b}f(x)d\alpha(x).$$
This is the Riemann-Stieltjes integral or simply the Stieltjes integral. Here we say that f is integrable with respect to $\alpha$, in the Riemann sense and write, $f\in\mathcal{R}(\alpha)$.
If $\alpha(x)=x$ then Riemann -Stieltjes integral becomes Riemann integral. Or we can say that Riemann integral is the special case of Riemann -Stieltjes integral.

---
### Theorem 1.2.1

> If $P^{*}$ is a refinement of P then
>
> $(i)U(P^{*},f,\alpha)\le U(P,f,\alpha)$
>
> $(ii)L(P,f,\alpha)\le L(P^{*},f,\alpha)$

**Proof:** Let $P=\{a=x_{0},x_{1},x_{2},...,x_{j-1},x_{j},...,x_{n}\}$
and $P^{*}=\{a=x_{0},x_{1},x_{2},...,x_{j-1},y,x_{j},...,x_{n}\}$
$m_{i}=inff(x)$ $x_{i-1}\le x\le x_{i}$
$M_{i}=sup~f(x)$ $x_{i-1}\le x\le x_{i}$
$W_{1}$ and $w_{1}$ be the supremum and infimum of f(x), $x\in[x_{j-1},y]$
$W_{2}$ and $w_{2}$ be the supremum and infimum of f(x), $x\in[y,x_{j}]$
Since sup $A\le sup~B$ and inf $A\ge inf~B$ whenever $A\subseteq B$
Here we have,
$[x_{j-1},y]\subseteq[x_{j-1},x_{j}]$ and $[y,x_{j}]\subseteq[x_{j-1},x_{j}]$
Therefore $W_{1}\le M_{j}$, $W_{2}\le M_{j}$, and $w_{1}\ge m_{j},w_{2}\ge m_{j}$ ... (1)

Since
$U(P^{*},f,\alpha)=\sum_{i=1}^{j-1}M_{i}\Delta\alpha_{i}+W_{1}[\alpha(y)-\alpha(x_{j-1})]+W_{2}[\alpha(x_{j})-\alpha(y)]+\sum_{i=j+1}^{n}M_{i}\Delta\alpha_{i}$
$U(\mathcal{P},f,\alpha)=\sum_{i=1}^{j-1}M_{i}\Delta\alpha_{i}+M_{j}\Delta\alpha_{j}+\sum_{i=j+1}^{n}M_{i}\Delta\alpha_{i}$
$U(P^{*},f,\alpha)-U(P,f,\alpha)=W_{1}[\alpha(y)-\alpha(x_{j-1})]+W_{2}[\alpha(x_{j})-\alpha(y)]-M_{j}\Delta\alpha_{j}$
$\le M_{j}[\alpha(x_{j})-\alpha(x_{j-1})]-M_{j}\Delta\alpha_{j}$ $\{by(1)\}$
$=M_{j}\Delta\alpha_{j}-M_{j}\Delta\alpha_{j}$
$=0$
$\Rightarrow U(P^{*},f,\alpha)-U(P,f,\alpha)\le 0$
$U(P^{*},f,\alpha)\le U(P,f,\alpha)$
This completes the proof of the first part.

Now we consider,
$L(\mathcal{P}^{*},f,\alpha)-L(\mathcal{P},f,\alpha)=w_{1}[\alpha(y)-\alpha(x_{j-1})]+w_{2}[\alpha(x_{j})-\alpha(y)]-m_{j}\Delta\alpha_{j}$
$\ge m_{j}[\alpha(y)-\alpha(x_{j-1})+\alpha(x_{j})-\alpha(y)]-m_{j}\Delta\alpha_{j}$
$=m_{j}\Delta\alpha_{j}-m_{j}\Delta\alpha_{j}$
$=0$
$\Rightarrow L(P^{*},f,\alpha)-L(P,f,\alpha)\ge0$
$\Rightarrow L(P,f,\alpha)\le L(P^{*},f,\alpha)$.
This completes the proof of the second part.

**Cor 1:** $\int_{\underline{a}}^{b}fd\alpha\le\int_{a}^{\overline{b}}fd\alpha$
**Proof:** Let $P^{*}=P_{1}\cup P_{2}$
$L(P_{1},f,\alpha)\le L(P^{*},f,\alpha)\le U(P^{*},f,\alpha)\le U(P_{2},f,\alpha)$
$\Rightarrow L(P_{1},f,\alpha)\le U(P_{2},f,\alpha)$
Keeping $P_{2}$ fixed and taking supremum over all partitions $P_{1}$, we get
$\int_{\underline{a}}^{b}fd\alpha\le U(P_{2},f,\alpha)$
Now by taking infimum over all partitions $P_{2},$ we get
$\Rightarrow\int_{\underline{a}}^{b}fd\alpha\le\int_{a}^{\overline{b}}fd\alpha.$

**Cor 2:** $L(\mathcal{P},f,\alpha)\le\int_{\underline{a}}^{b}fd\alpha$ and $U(\mathcal{P},f,\alpha)\ge\int_{a}^{\overline{b}}fd\alpha$
Also, we have $\int_{\underline{a}}^{b}fd\alpha\le\int_{a}^{\overline{b}}fd\alpha$
Therefore,
$L(P,f,\alpha)\le\int_{\underline{a}}^{b}fd\alpha\le\int_{a}^{\overline{b}}fd\alpha\le U(P,f,\alpha)$
If $f\in\mathcal{R}(\alpha)$ then $\int_{a}^{b}fd\alpha = \int_{\underline{a}}^{b}fd\alpha = \int_{a}^{\overline{b}}fd\alpha$
So $L(\mathcal{P},f,\alpha)\le\int_{a}^{b}fd\alpha\le U(\mathcal{P},f,\alpha)$

**Cor 3:** If $f\in\mathcal{R}(\alpha)$ on $[a,b]$ and m, M are the lower and upper bounds of f defined on [a, b] then
$m[\alpha(b)-\alpha(a)]\le\int_{a}^{b}fd\alpha\le M[\alpha(b)-\alpha(a)]$
Since,
$m[\alpha(b)-\alpha(a)]\le L(P,f,\alpha)\le U(P,f,\alpha)\le M[\alpha(b)-\alpha(a)]$
and
$L(P,f,\alpha)\le\int_{a}^{b}fd\alpha\le U(P,f,\alpha)$
$\therefore m[\alpha(b)-\alpha(a)]\le L(P,f,\alpha)\le\int_{a}^{b}fd\alpha\le U(P,f,\alpha)\le M[\alpha(b)-\alpha(a)]$
$\Rightarrow m[\alpha(b)-\alpha(a)]\le\int_{a}^{b}fd\alpha\le M[\alpha(b)-\alpha(a)].$

---
### Theorem 1.2.2

> Let f and $\alpha$ be bounded functions on [a, b] and $\alpha$ be monotonically increasing on [a, b]. Then $f\in\mathcal{R}(\alpha)$ if and only if for every $\epsilon>0,$ there exists a partition of [a, b]such that $U(P,f,\alpha)-L(P,f,\alpha)<\epsilon.$

**Proof:** Suppose $f\in\mathcal{R}(\alpha)$
$\therefore\int_{\underline{a}}^{b}fd\alpha=\int_{a}^{\overline{b}}fd\alpha=\int_{a}^{b}fd\alpha$
Let $\epsilon>0$ be any number.
Since $inf_{P}U(P,f,\alpha)=\int_{a}^{\overline{b}}fd\alpha$
$\Rightarrow\int_{a}^{\overline{b}}fd\alpha+\frac{\epsilon}{2}$ is not the lower bound of this set.
So there exists a partition $P_{1}$ of [a, b] such that
$U(P_{1},f,\alpha)<\int_{a}^{\overline{b}}fd\alpha+\frac{\epsilon}{2}$
$=\int_{a}^{b}fd\alpha+\frac{\epsilon}{2}$ $f\in\mathcal{R}(\alpha)$
$\therefore U(P_{1},f,\alpha)<\int_{a}^{b}fd\alpha+\frac{\epsilon}{2}$ ...(1)

Further,
$sup_{P}L(P,f,\alpha)=\int_{\underline{a}}^{b}fd\alpha$
$\Rightarrow\int_{\underline{a}}^{b}fd\alpha-\frac{\epsilon}{2}$ can not be the upper bound of this set.
$\therefore$ there exists a partition $P_{2}$ of [a, b] such that
$L(P_{2},f,\alpha)>\int_{\underline{a}}^{b}fd\alpha-\frac{\epsilon}{2}$
$\Rightarrow\int_{a}^{b}fd\alpha<L(P_{2},f,\alpha)+\frac{\epsilon}{2}$

Let $P=P_{1}\cup P_{2}$
Now,
$U(P,f,\alpha)\le U(P_{1},f,\alpha)$
$<\int_{a}^{b}fd\alpha+\frac{\epsilon}{2}$ {by(1)}
$<L(P_{2},f,\alpha)+\frac{\epsilon}{2}+\frac{\epsilon}{2}$ {by(2)}
$\le L(P,f,\alpha)+\epsilon$ as $P$ is the refinement of $P_{2}$
$\Rightarrow U(P,f,\alpha)-L(P,f,\alpha)<\epsilon.$

Conversely, let $U(P,f,\alpha)-L(P,f,\alpha)<\epsilon$
We also have
$L(\mathcal{P},f,\alpha)\le\int_{\underline{a}}^{b}fd\alpha\le\int_{a}^{\overline{b}}fd\alpha\le U(\mathcal{P},f,\alpha)$
$\Rightarrow\int_{a}^{\overline{b}}fd\alpha-\int_{\underline{a}}^{b}fd\alpha\le U(\mathcal{P},f,\alpha)-L(\mathcal{P},f,\alpha)$
$<\epsilon$
$\Rightarrow0\le\int_{a}^{\overline{b}}fd\alpha-\int_{\underline{a}}^{b}fd\alpha\le\epsilon$
$\Rightarrow\int_{a}^{\overline{b}}fd\alpha=\int_{\underline{a}}^{b}fd\alpha$
$\Rightarrow f\in\mathcal{R}(\alpha)$
This completes the proof.

**Cor:** If $U(P,f,\alpha)-L(P,f,\alpha)<\epsilon$ for some partition P then this result holds for every refinement $P^{*}$ of P.
**Proof:** We have,
$U(P^{*},f,\alpha)\le U(P,f,\alpha)$
and
$L(P^{*},f,\alpha)\ge L(P,f,\alpha)$
$\Rightarrow-L(P^{*},f,\alpha)\le-L(P,f,\alpha)$
Therefore,
$U(P^{*},f,\alpha)-L(P^{*},f,\alpha)\le U(P,f,\alpha)-L(P,f,\alpha)$
$<\epsilon$
Thus, we get
$U(P^{*},f,\alpha)-L(P^{*},f,\alpha)<\epsilon$

---
### Theorem 1.2.3

> If f is a constant function defined by $f(x)=k$ $\forall x \in [a,b]$ and $\alpha$ is monotonically increasing function on [a, b] then $\int_{a}^{b}fd\alpha$ exists and is equal to $k[\alpha(b)-\alpha(a)]$.

**Proof:** Let $P=\{a=x_{0},x_{1},x_{2},...,x_{n}=b\}$ be the partition of [a, b] such that $x_{0}\le x_{1}\le x_{2}\le\cdot\cdot\cdot\le x_{n}$
$m_{i}=inff(x),x_{i-1}\le x\le x_{i},$
$M_{i}=sup~f(x),x_{i-1}\le x\le x_{i}$
Since $f(x)=k\forall x\in[a,b].$
Therefore, $m_{i}=M_{i}=k\forall i$
Now
$U(P,f,\alpha)=\sum_{i=1}^{n}M_{i}\Delta\alpha_{i}$
$=k\sum_{i=1}^{n}\Delta\alpha_{i}$
$=k[\alpha(b)-\alpha(a)]$
and $L(\mathcal{P},f,\alpha)=\sum_{i=1}^{n}m_{i}\Delta\alpha_{i}$
$=k\sum_{i=1}^{n}\Delta\alpha_{i}$
$=k[\alpha(b)-\alpha(a)]$

$\int_{\underline{a}}^{b}fd\alpha=sup_{P}L(P,f,\alpha)$
$=sup_{P}k[\alpha(b)-\alpha(a)]$
$=k[\alpha(b)-\alpha(a)]$
$\int_{a}^{\overline{b}}fd\alpha=inf_{P}U(P,f,\alpha)$
$=inf_{P}k[\alpha(b)-\alpha(a)]$
$=k[\alpha(b)-\alpha(a)]$
Thus, we get
$\int_{\underline{a}}^{b}fd\alpha=\int_{a}^{\overline{b}}fd\alpha=k[\alpha(b)-\alpha(a)]$
$\Rightarrow\int_{a}^{b}fd\alpha=k[\alpha(b)-\alpha(a)]$
This completes the proof.

---
### Theorem 1.2.4

> If $U(P,f,\alpha)-L(P,f,\alpha)<\epsilon$ for a partition P of [a, b] and if $s_{i}$ and $t_{i}$ are arbitrary points of $[x_{i-1},x_{i}]$ then
> $\sum_{i=1}^{n}|f(s_{i})-f(t_{i})|\Delta\alpha_{i}<\epsilon.$

**Proof:** Let $m_{i}=inff(x),x_{i-1}\le x\le x_{i},$
$M_{i}=sup~f(x),x_{i-1}\le x\le x_{i}$
Since $s_{i}, t_{i}\in[x_{i-1},x_{i}]$
Therefore,
$f(s_{i}),f(t_{i})\in[m_{i},M_{i}]$
$\Rightarrow|f(s_{i})-f(t_{i})|\le M_{i}-m_{i}$
$\sum_{i=1}^{n}|f(s_{i})-f(t_{i})|\Delta\alpha_{i} \le \sum_{i=1}^{n}(M_{i}-m_{i})\Delta\alpha_{i}$
$\le\sum_{i=1}^{n}M_{i}\Delta\alpha_{i}-\sum_{i=1}^{n}m_{i}\Delta\alpha_{i}$
$=U(P,f,\alpha)-L(P,f,\alpha)$
$<\epsilon$
Thus, we get
$\sum_{i=1}^{n}|f(s_{i})-f(t_{i})|\Delta\alpha_{i}<\epsilon.$
This completes the proof.

---
### Theorem 1.2.5

> If $f\in\mathcal{R}(\alpha)$ on [a, b] then for every $\epsilon > 0$, there exists a partition
> $P=\{a=x_{0},x_{1},x_{2},...,x_{n}=b\}$ of [a, b] such that
> $|\sum_{i=1}^{n}f(t_{i})\Delta\alpha_{i}-\int_{a}^{b}fd\alpha|<\epsilon,t_{i}\in[x_{i-1},x_{i}].$

**Proof:** Since $f\in\mathcal{R}(\alpha)$ on [a, b], therefore for given $\epsilon>0,$ there exists a partition P of [a, b] such that
$U(P,f,\alpha)-L(P,f,\alpha)<\epsilon$
Let $m_{i}=inff(x),x_{i-1}\le x\le x_{i},$
$M_{i}=supf(x),x_{i-1}\le x\le x_{i}$
$sincet_{i}\in[x_{i-1},x_{i}]$
$\Rightarrow f(t_{i})\in[m_{i},M_{i}]$
$\Rightarrow m_{i}\le f(t_{i})\le M_{i}$
$\sum_{i=1}^{n}m_{i}\Delta\alpha_{i}\le\sum_{i=1}^{n}f(t_{i})\Delta\alpha_{i}\le\sum_{i=1}^{n}M_{i}\Delta\alpha_{i}$
$L(\mathcal{P},f,\alpha)\le\sum_{i=1}^{n}f(t_{i})\Delta\alpha_{i}\le U(\mathcal{P},f,\alpha)$ ... (1)
We also have,
$L(P,f,\alpha)\le\int_{a}^{b}fd\alpha\le U(P,f,\alpha)$ ... (2)
Thus, using relations (1) and (2), we get
$|\sum_{i=1}^{n}f(t_{i})\Delta\alpha_{i}-\int_{a}^{b}fd\alpha|<U(\mathcal{P},f,\alpha)-L(\mathcal{P},f,\alpha)$
$<\epsilon.$
Thus, we get
$|\sum_{i=1}^{n}f(t_{i})\Delta\alpha_{i}-\int_{a}^{b}fd\alpha|<\epsilon,t_{i}\in[x_{i-1},x_{i}],$
This completes the proof.

---
### Theorem 1.2.6

> If f is a continuous function on [a, b] then $f\in\mathcal{R}(\alpha)$, $\alpha$ is monotonically increasing function on [a, b].

**Proof:** Let $\epsilon>0$ and choose $\eta>0$ such that $[\alpha(b)-\alpha(a)]\eta<\epsilon$.
Since f is continuous on [a, b] therefore f is uniformly continuous on [a, b].
For above $\eta>0,$ there exits $\delta>0$ such that $|f(x)-f(y)|<\eta$ whenever $|x-y|<\delta$, $\forall x,y\in[a,b]$.
Consider partition P of [a, b] such that $||P||<\delta$
$||P||=Max\{\Delta x_{1},\Delta x_{2},...,\Delta x_{n}\}$
$\Rightarrow\Delta x_{i}<\delta$ $\forall i$
f is continuous on [a, b], therefore f is bounded and attains its bound on [a, b].
Therefore, there exist numbers $c_{i}, d_{i}\in[x_{i-1},x_{i}]$ such that $f(c_{i})=m_{i}=inff(x)$
$f(d_{i})=M_{i}=sup~f(x)$
$M_{i}-m_{i}=|M_{i}-m_{i}|$
$=|f(d_{i})-f(c_{i})|$
$\because|d_{i}-c_{i}|\le|x_{i}-x_{i-1}|<\delta,$
Thus $|d_{i}-c_{i}|<\delta\Rightarrow|f(d_{i})-f(c_{i})|<\eta.$
$M_{i}-m_{i} < \eta$
$U(\mathcal{P},f,\alpha)-L(\mathcal{P},f,\alpha)=\sum_{i=1}^{n}M_{i}\Delta\alpha_{i}-\sum_{i=1}^{n}m_{i}\Delta\alpha_{i}$
$=\sum_{i=1}^{n}(M_{i}-m_{i})\Delta\alpha_{i}$
$<\sum_{i=1}^{n}\eta~\Delta\alpha_{i}$
$=\eta\sum_{i=1}^{n}\Delta\alpha_{i}$
$=\eta[\alpha(b)-\alpha(a)]<\epsilon$
$\Rightarrow U(P,f,\alpha)-L(P,f,\alpha)<\epsilon$
$\Rightarrow f\in\mathcal{R}(\alpha)$
This completes the proof.

---
### Theorem 1.2.7

> If f is monotonic on [a, b] and $\alpha$ is continuous and monotonically increasing then $f\in\mathcal{R}(\alpha)$.

**Proof:** Since $\alpha$ is a continuous and monotonically increasing function.
for every positive integer $n$, we can find a partition P such that
$\Delta\alpha_{i}=\frac{\alpha(b)-\alpha(a)}{n},i=1,2,...n.$
Define
$m_{i}=inf~f(x)$, $x_{i-1}\le x\le x_{i}$
$=f(x_{i-1})$
$M_{i}=sup~f(x)$, $x_{i-1}\le x\le x_{i}$
$=f(x_{i})$.
Now,
$U(\mathcal{P},f,\alpha)-L(\mathcal{P},f,\alpha)=\sum_{i=1}^{n}(M_{i}-m_{i})\Delta\alpha_{i}$
$=\frac{\alpha(b)-\alpha(a)}{n}\sum_{i=1}^{n}(M_{i}-m_{i})$
$=\frac{\alpha(b)-\alpha(a)}{n}\sum_{i=1}^{n}(f(x_{i})-f(x_{i-1}))$
$=\frac{\alpha(b)-\alpha(a)}{n}(f(b)-f(a))$
$<\epsilon$ when $n\rightarrow\infty$
$\Rightarrow U(P,f,\alpha)-L(P,f,\alpha)<\epsilon\Rightarrow f\in\mathcal{R}(\alpha)$

---
### Examples

**Example:** If $f(x)=x^{2}$ and $\alpha(x)=x^{3}$ then evaluate $\int_{a}^{b}f~d\alpha,a=0,b=1.$
**Solution:** $\int_{a}^{b}fd\alpha$
$=\int_{0}^{1}x^{2}d(x^{3})$
$=\int_{0}^{1}x^{2}(3x^{2})dx$
$=3\int_{0}^{1}x^{4}dx$
$=3[\frac{x^{5}}{5}]_{0}^{1}$
$=\frac{3}{5}$

**Example:** Evaluate $\int_{0}^{3}x~d([x]-x)$
**Solution:** We have
$\int_{0}^{3}x~d([x]-x)$
$=\int_{0}^{3}x~d[x]-\int_{0}^{3}x\cdot dx$
$=1+2+3-[\frac{x^{2}}{2}]_{0}^{3}$
$=6-\frac{9}{2}=\frac{12-9}{2}=\frac{3}{2}$

**Example:** Evaluate $\int_{0}^{3}e^{x}d\{x-[x]\}$
**Solution:** We have
$\int_{0}^{3}e^{x}d\{x-[x]\}$
$=\int_{0}^{3}e^{x}dx-\int_{0}^{3}e^{x}d[x]$
$=[e^{x}]_{0}^{3}-(e+e^{2}+e^{3})$
$=e^{3}-1-e-e^{2}-e^{3}$
$=-(1+e+e^{2})$

**Example:** Evaluate $\int_{0}^{6}\{x^{2}+[x]\}d(|3-x|)$
**Solution:** We have
$|3-x|=\begin{cases}3-x&if~3-x\ge0~i.e.x\le3\\ -(3-x)&if~3-x<0~i.e.x>3\end{cases}$
$\therefore\int_{0}^{6}\{x^{2}+[x]\}d(|3-x|)=\int_{0}^{3}\{x^{2}+[x]\}d(3-x)+\int_{3}^{6}\{x^{2}+[x]\}d(x-3)$
$=-\int_{0}^{3}\{x^{2}+[x]\}dx+\int_{3}^{6}\{x^{2}+[x]\}dx$
$=-[\int_{0}^{3}x^{2}dx+\int_{0}^{3}[x]dx]+\int_{3}^{6}x^{2}dx+\int_{3}^{6}[x]dx$
$=-[\int_{0}^{3}x^{2}dx+\int_{0}^{1}[x]dx+\int_{1}^{2}[x]dx+\int_{2}^{3}[x]dx]+\int_{3}^{6}x^{2}dx+\int_{3}^{4}[x]dx+\int_{4}^{5}[x]dx+\int_{5}^{6}[x]dx$
$=-\{[\frac{x^{3}}{3}]_{0}^{3}+1+2\}+[\frac{x^{3}}{3}]_{3}^{6}+3+4+5=63$

**Example:** Evaluate $\int_{\pi}^{2\pi}sin~x~d(cos~x)$
**Solution:** We have,
$\int_{\pi}^{2\pi}sin~x~d(cos~x)$
$=\int_{\pi}^{2\pi}sin~x(-sin~x)dx$
$=-\int_{\pi}^{2\pi}sin^{2}x~dx$
$=-\int_{\pi}^{2\pi}\frac{1-cos~2x}{2}dx$
$=\frac{1}{2}\int_{\pi}^{2\pi}(cos~2x-1)dx$
$=\frac{1}{2}[\frac{sin~2x}{2}-x]_{\pi}^{2\pi}$
$=-\frac{\pi}{2}$

---
### Theorem 1.2.8

> Let $f\in\mathcal{R}(\alpha)$ on [a,b] and $m\le f(x)\le M$ $\forall x\in [a, b]$. Let $\Phi: [m,M]\rightarrow\mathbb{R}$ be continuous function. Then $h=\Phi\circ f\in\mathcal{R}(\alpha)$ on $[a,b].$

**Proof:** Let $\epsilon>0$ be given. As $\Phi$ is continuous in $[m,M]$ therefore $\Phi$ is uniformly continuous in $[m, M]$.
So for given $\epsilon>0$ $\exists \delta>0$ such that
$|\Phi(s)-\Phi(t)|<\epsilon$ $\forall s,t\in[m,M]$ whenever $|s-t|<\delta$
We assume $\delta<\epsilon$
Since $f\in\mathcal{R}(\alpha)$ on[a, b].
for given $\delta > 0$, $\exists$ a partition
$P=\{a=x_{0},x_{1},x_{2},...x_{n}=b\}$ of [a, b] such that
$U(P,f,\alpha)-L(P,f,\alpha)<\delta^{2}$ ...(1)
Let
$m_{i}=inf\{f(x):x\in[x_{i-1},x_{i}]\}$
$M_{i}=sup\{f(x):x\in[x_{i-1},x_{i}]\}$
$m_{i}^{\prime}=inf\{h(x):x\in[x_{i-1},x_{i}]\}$
$M_{i}^{\prime}=sup\{h(x):x\in[x_{i-1},x_{i}]\}$
Divide the numbers $i=1.2,...,n$ into two classes A and B where
$A=\{i:M_{i}-m_{i}<\delta\}$ and $B=\{i:M_{i}-m_{i}\ge\delta\}$
when $i\in A$ and $x_{i-1}\le x<y\le x_{i}$ we have
$|f(x)-f(y)|\le M_{i}-m_{i}<\delta$
$\Rightarrow|\Phi(f(x))-\Phi(f(y))|<\epsilon$ (by (1))
$\Rightarrow|h(x)-h(y)|<\epsilon$
$\Rightarrow M_{i}^{\prime}-m_{i}^{\prime}\le\epsilon$
$i.e.M_{i}^{\prime}-m_{i}^{\prime}\le\epsilon$ when $i \in A$
$\therefore\sum_{i\in A}(M_{i}^{\prime}-m_{i}^{\prime})\Delta\alpha_{i}\le\sum_{i\in A}\epsilon~\Delta\alpha_{i}$
$=\epsilon\sum_{i\in A}\Delta\alpha_{i}$
$\le\epsilon[\alpha(b)-\alpha(a)]$
$\therefore\sum_{i\in A}(M_{i}^{\prime}-m_{i}^{\prime})\Delta\alpha_{i}<\epsilon[\alpha(b)-\alpha(a)]$ (3)

Now
$\delta\sum_{i\in B}\Delta\alpha_{i}\le\sum_{i\in B}(M_{i}-m_{i})\Delta\alpha_{i}$
$\le\sum_{i}(M_{i}-m_{i})\Delta\alpha_{i}$
$=U(P,f,\alpha)-L(P,f,\alpha)$
$<\delta^{2}$ (Using (1))
$\therefore\sum_{i\in B}\Delta\alpha_{i}<\delta<\epsilon$ .......(4)
Also, for $i\in B$, we have
$M_{i}^{\prime}-m_{i}^{\prime}=|M_{i}^{\prime}-m_{i}^{\prime}|$
$\le|M_{i}^{\prime}|+|m_{i}^{\prime}|$
$\le k+k=2k$ ... (5)
Where $k=sup|\Phi(t)|$, $m\le t\le M$
$U(P,h,\alpha)-L(P,h,\alpha)=\sum_{i}(M_{i}^{\prime}-m_{i}^{\prime})\Delta\alpha_{i}$
$=\sum_{i\in A}(M_{i}^{\prime}-m_{i}^{\prime})\Delta\alpha_{i}+\sum_{i\in B}(M_{i}^{\prime}-m_{i}^{\prime})\Delta\alpha_{i}$
$<\epsilon[\alpha(b)-\alpha(a)]+2k\epsilon$ (by(3),(4),(5))
$=[\alpha(b)-\alpha(a)+2k]\epsilon=\epsilon^{\prime}$
$\Rightarrow U(P,h,\alpha)-L(P,h,\alpha)<\epsilon^{\prime}$
$\Rightarrow h\in\mathcal{R}(\alpha)$ on $[a,b].$
This completes the proof.

**Cor:** If $f\in\mathcal{R}(\alpha)$ on [a, b] then $f^{2}\in\mathcal{R}(\alpha)$ and $|f|\in\mathcal{R}(\alpha).$
Let $\Phi(t)=t^{2}$ so that $\Phi$ is continuous on [m, M] then $\Phi\circ f\in\mathcal{R}(\alpha)$ on [a, b].
Now
$(\Phi\circ f)(x)=\Phi(f(x))$
$=[f(x)]^{2}$
$\Rightarrow f^{2}\in\mathcal{R}(\alpha)$ on [a,b].
Again let,
$\Phi(t)=|t|$ so that $\Phi$ is continuous on [m, M] then $\Phi\circ f\in\mathcal{R}(\alpha)$ on [a, b].
Now
$(\Phi\circ f)(x)=\Phi(f(x))=|f(x)|$
$|f|\in\mathcal{R}(\alpha)$ on [a, b].
